---
title: Matrix exponential
parent: Reference
nav_order: 3
---

# The matrix exponential function
{: .no_toc }

- TOC
{:toc }

## What is the matrix exponential?

The **matrix exponential** of a square matrix $M$ is the infinite series

$$
e^M = I + M + \frac{1}{2}M^2 + \frac{1}{6}M^3 + \dotsm = \sum_{k=0}^{\infty} \dfrac{1}{k !} M^k
$$

where $I$ is the identity matrix. This series converges for any square matrix $M$.


## How do I use the matrix exponential to solve a linear system?

The solution to the set of linear ODEs

$$ \dot{x} = Fx $$

with the initial condition

$$ x(t_0) = x_0 $$

is

$$ x(t) = e^{F (t - t_0)} x_0. $$

How do we know that this solution is correct? First, let's check that this solution satisfies the ODEs:

$$
\begin{aligned}
\dot{x}
&= \frac{d}{dt} \left( e^{F (t - t_0)} x_0 \right) \\
&= \frac{d}{dt} \left( \left( I + F(t-t_0) + \frac{1}{2} F^2(t-t_0)^2 + \frac{1}{6} F^2(t-t_0)^3 + \dotsm \right) x_0 \right) \\
&= \frac{d}{dt} \left( I + F(t-t_0) + \frac{1}{2} F^2(t-t_0)^2 + \frac{1}{6} F^3(t-t_0)^3 + \dotsm \right) x_0 \\
&= \left( \frac{d}{dt} \left( I \right) + \frac{d}{dt} \left( F(t-t_0) \right) + \frac{d}{dt} \left( \frac{1}{2} F^2(t-t_0)^2 \right) + \frac{d}{dt} \left( \frac{1}{6} F^3(t-t_0)^3 \right) \dotsm \right) x_0 \\
&= \left( 0 + F + F^2(t-t_0) + \frac{1}{2} F^3(t-t_0) + \dotsm \right) x_0 \\
&= F \left(I + F(t-t_0) + \frac{1}{2} F^2(t-t_0)^2 + \dotsm \right) x_0 \\
&= F e^{F(t-t_0)} x_0
\end{aligned}
$$

Apparently, it does. Second, let's check that this solution satisfies the initial condition:

$$ \begin{aligned} x(t_0) &= e^{F(t_0 - t_0)} x_0 \\ &= e^0 x_0 \\ &= I x_0 \\ &= x_0 \end{aligned} $$

Again, it does. (We might wonder if this is the *only* solution to the original ODEs --- it is, although a proof would require more work.)

## How do I use the matrix exponential to solve state space models?

Consider the state space model

$$ \dot{x} = Ax + Bu$$

This model does not look the same as

$$ \dot{x} = Fx $$

Indeed, without specifying $u$, we cannot solve for $x$ as a function of time. However, particular choices of $u$ allow us to simplify the state space model. For example, if we choose $u = 0$, then we can write

$$ \begin{aligned} \dot{x} &= Ax+Bu \\ &= Ax + B \cdot (0) \\ &= Ax + 0 \\ &= Ax \end{aligned} $$

and so we are right back at a linear system that can be solved with the matrix exponential. Another common choice of $u$ is

$$ u = -Kx $$

for some constant matrix $K$. (What would the size of $K$ have to be for us to define $u$ in this way?) This choice of $u$ is called **state feedback**, since the input depends on the state. If we plug this choice into our state space model, then we can write

$$
\begin{aligned}
\dot{x} &= Ax + Bu \\
&= Ax + B(-Kx) \\
&= (A - BK) x
\end{aligned}
$$

and so --- just like before --- we are right back at a linear system that can be solved with the matrix exponential. Although this result will get us a long way, we will see how to solve state space models for other choices of input later on.

{: .note }
> Given the state-space model
> 
> $$\dot{x} = Ax + Bu$$
> 
> it is standard to call the system
> 
> $$\dot{x} = Ax$$
> 
> that results from the application of zero input $u=0$ the **open-loop system**. Similarly, it is standard to call the system
> 
> $$\dot{x} = (A - BK) x$$
> 
> that results from the application of linear state feedback $u = -Kx$ the **closed-loop system**. Remember that "zero input" is not necessarily the same as "zero actuator commands." When [linearizing equations of motion to derive a state space model](state-space-models#how-do-i-put-a-system-in-state-space-form), we defined
> 
> $$u = n - n_e$$
> 
> where $n$ was the set of actuator commands and $n_e$ was the value of these commands at equilibrium. So,
> 
> $$u = 0$$
> 
> actually means
> 
> $$n = n_e.$$
> 
> Similarly,
> 
> $$u = -Kx$$
> 
> actually means
> 
> $$n = n_e - Kx = n_e - K(m - m_e).$$
> 
> The term $n_e$ is typically referred to as **feedforward** and the term $-K(m - m_e)$ is typically referred to as **feedback**.